lib/Base/Functional.i.dfy
@@ -1,0 +1,5 @@
+module Functional {
+  predicate ImpliesRequires<D(!new),R>(p: D -> bool, f: D --> R) {
+    forall x | p(x) :: f.requires(x)
+  }
+}
